src/Framework/Base.v
@@ -1,0 +1,56 @@
+From Coq Require Import ZArith.ZArith Sets.Ensembles Lists.List.
+From compcert.lib Require Export Maps.
+From Hammer Require Import Hammer Tactics Reflect.
+
+Module M := Maps.PTree.
+Definition var := M.elt.
+Definition vars := Ensemble var.
+
+(* Constructor Tags *)
+Definition ctor_tag := M.elt.
+
+Inductive find_tag {exp : Type} : list (ctor_tag * exp) -> ctor_tag -> exp -> Prop :=
+| find_tag_hd :
+  forall c e l,
+    find_tag ((c, e) :: l) c e
+
+| find_tag_tl :
+  forall c e l c' e',
+    find_tag l c' e' ->
+    c <> c' ->
+    find_tag ((c, e) :: l) c' e'.
+
+Hint Constructors find_tag : core.
+
+Lemma find_tag_deterministic {exp : Type} {cl c} {e e' : exp} :
+  find_tag cl c e ->
+  find_tag cl c e' ->
+  e = e'.
+Proof.
+  intros H. revert e'.
+  induction H; sauto.
+Qed.
+
+(* Label *)
+Definition label := M.elt.
+Definition labels := Ensemble label.
+Definition next_label l : label := Pos.succ l.
+
+Lemma next_label_lt l : Pos.lt l (next_label l).
+Proof.
+  unfold next_label.
+  eapply Pos.lt_succ_diag_r; eauto.
+Qed.
+
+Lemma next_label_le l : Pos.le l (next_label l).
+Proof.
+  eapply Pos.lt_le_incl; eauto.
+  eapply next_label_lt; eauto.
+Qed.
+
+(* Fuel *)
+Definition fuel := nat.
+
+(* Web Identifiers *)
+Definition web := M.elt.
+Definition webs := Ensemble web.
